\section*{Problem 3}
\setcounter{section}{3}
\setcounter{equation}{0}

\textbf{Passivity of Robot Dynamics:} \\
Let \( \mathcal{H}(\theta)=\mathcal{T}(\theta)+\mathcal{V}(\theta) \) be the total energy for a rigid robot.
Show that if \( \dot{\mathcal{M}}-2 \mathcal{C} \) is skew-symmetric, then energy is conserved, i.e., \( \dot{\mathcal{H}}=\dot{\theta}^{\top} \tau \).
(Basically total energy only changes due to the input work applied to the system.).

\subsection*{Solution}

Given that \( \mathcal{H}(\theta)=\mathcal{T}(\theta)+\mathcal{V}(\theta) \) is the total energy for a rigid robot, we have the kinetic energy as
\begin{equation*}
    \mathcal{T}(\theta)
    =
    \frac{1}{2} \dot{\theta}^{\top} \mathcal{M}(\theta) \dot{\theta}
\end{equation*}
\begin{align*}
    \implies
    \dot{\mathcal{T}}
     & =
    \frac{1}{2} \left( \ddot{\theta}^{\top} \mathcal{M}(\theta) \dot{\theta}+\dot{\theta}^{\top} \mathcal{M}(\theta) \ddot{\theta} \right)
    \\
    \implies
    \dot{\mathcal{H}}
     & =
    \dot{\mathcal{T}}+\dot{\mathcal{V}}
    =
    \frac{1}{2} \ddot{\theta}^{\top} \mathcal{M}(\theta) \dot{\theta}
    +
    \frac{1}{2} \dot{\theta}^{\top} \mathcal{M}(\theta) \ddot{\theta}
    +
    \frac{\partial \mathcal{V}(\theta)}{\partial \theta} \dot{\theta}
\end{align*}
The dynamics of a rigid robot are given by
\begin{equation*}
    \mathcal{M}(\theta) \ddot{\theta}+\mathcal{C}(\theta, \dot{\theta}) \dot{\theta}+\mathcal{G}(\theta)=\tau
\end{equation*}
where \( \mathcal{M}(\theta) \) is the inertia matrix, \( \mathcal{C}(\theta, \dot{\theta}) \) is the Coriolis matrix, \( \mathcal{G}(\theta) \) is the gravity matrix, and \( \tau \) is the control input.
Now, we have
\begin{align*}
    \implies
    \mathcal{M}(\theta) \ddot{\theta}
     & =
    \tau-\mathcal{C}(\theta, \dot{\theta}) \dot{\theta}-\mathcal{G}(\theta)
    \\
    \implies
    \dot{\mathcal{H}}
     & =
    \frac{1}{2} \ddot{\theta}^{\top} \mathcal{M}(\theta) \dot{\theta}
    +
    \frac{1}{2} \dot{\theta}^{\top} \left( \tau-\mathcal{C}(\theta, \dot{\theta}) \dot{\theta}-\mathcal{G}(\theta) \right)
    +
    \frac{\partial \mathcal{V}(\theta)}{\partial \theta} \dot{\theta}
    \\
    \because
    \mathcal{G}(\theta)
     & =
    -\frac{\partial \mathcal{V}(\theta)}{\partial \theta}
    \\
    \implies
    \dot{\mathcal{H}}
     & =
    \dot{\theta}^{\top} \tau-\dot{\theta}^{\top} \mathcal{C}(\theta, \dot{\theta}) \dot{\theta}-\dot{\theta}^{\top} \mathcal{G}(\theta) + \dot{\mathcal{V}}
\end{align*}
Given that \( \dot{\mathcal{M}}-2 \mathcal{C} \) is skew-symmetric, we have
\begin{align*}
    \left( \dot{\mathcal{M}}-2 \mathcal{C} \right)^{\top}
     & =
    -\left( \dot{\mathcal{M}}-2 \mathcal{C} \right)
    \implies
    \dot{\mathcal{M}}^{\top}-2 \mathcal{C}^{\top}
    =
    -\dot{\mathcal{M}}+2 \mathcal{C}
\end{align*}
Since \( \mathcal{M} \) is symmetric and positive definite, we have \( {\mathcal{M}}^{\top} = \mathcal{M} \implies \dot{\mathcal{M}}^{\top} = \dot{\mathcal{M}} \).
