\section*{Problem 1}

Show that the adjoint transformation \( \operatorname{Ad}_{g}: \mathbb{R}^{6} \mapsto \mathbb{R}^{6} \) given below is invertible and compute its inverse.
\[
    \operatorname{Ad}_{g}=\left[\begin{array}{cc}
            R & \widehat{p} R \\
            0 & R
        \end{array}\right], \text { where, } g \equiv(p, R) \in SE(3)
\]

\subsection*{Solution}

Given \( g \in SE(3) \), we can write \( g \) as \( g = (p, R) \), where \( p \in \mathbb{R}^{3} \) and \( R \in SO(3) \). The adjoint transformation \( \operatorname{Ad}_{g}: \mathbb{R}^{6} \mapsto \mathbb{R}^{6} \) is defined by
\begin{equation*}
    \operatorname{Ad}_{g}
    =
    \begin{bmatrix}
        R & \widehat{p} R \\
        0 & R
    \end{bmatrix}_{6 \times 6}
\end{equation*}

To show that \( \operatorname{Ad}_{g} \) is invertible, we need to show that \( \operatorname{Ad}_{g} \) is a square matrix and that its determinant is non-zero.
The matrix \( \operatorname{Ad}_{g} \) is a \( 6 \times 6 \) matrix, and its determinant is given by
\begin{equation*}
    \det(\operatorname{Ad}_{g})
    =
    \det
    \begin{bmatrix}
        R & \widehat{p} R \\
        0 & R
    \end{bmatrix}
    =
    \det( R R - \widehat{p} R \cdot 0 )
    =
    \det(R^{2})
    =
    \det(R) \det(R)
    =
    1
\end{equation*}
where we considered the matrices as block matrices.
Thereby, the inverse of \( \operatorname{Ad}_{g} \) exists, and is given by
\begin{equation*}
    \boxed{
    \operatorname{Ad}_{g}^{-1}
    =
    \begin{bmatrix}
        R^{-1} & -R^{-1} \widehat{p} \\
        0      & R^{-1}
    \end{bmatrix}_{6 \times 6}
    =
    \begin{bmatrix}
        R^{T} & -R^{T} \widehat{p} \\
        0     & R^{T}
    \end{bmatrix}
    }
\end{equation*}

We can indeed verify that this is the inverse, by
\begin{align*}
    \operatorname{Ad}_{g}^{-1}
    \operatorname{Ad}_{g}
     & =
    \begin{bmatrix}
        R^{T} & -R^{T} \widehat{p} \\
        0     & R^{T}
    \end{bmatrix}
    \begin{bmatrix}
        R & \widehat{p} R \\
        0 & R
    \end{bmatrix}
    =
    \begin{bmatrix}
        R^{T} R & R^{T} \widehat{p} R - R^{T} \widehat{p} R \\
        0       & R^{T} R
    \end{bmatrix}
    =
    \begin{bmatrix}
        I_{3 \times 3} & 0              \\
        0              & I_{3 \times 3}
    \end{bmatrix}
    =
    I_{6 \times 6}
    \\
    \operatorname{Ad}_{g}
    \operatorname{Ad}_{g}^{-1}
     & =
    \begin{bmatrix}
        R & \widehat{p} R \\
        0 & R
    \end{bmatrix}
    \begin{bmatrix}
        R^{T} & -R^{T} \widehat{p} \\
        0     & R^{T}
    \end{bmatrix}
    =
    \begin{bmatrix}
        R R^{T} & -R R^{T} \widehat{p} + \widehat{p} R R^T \\
        0       & R R^{T}
    \end{bmatrix}
    \\ & =
    \begin{bmatrix}
        I_{3 \times 3} & - \widehat{p} + \widehat{p} \\
        0              & I_{3 \times 3}
    \end{bmatrix}
    =
    \begin{bmatrix}
        I_{3 \times 3} & 0              \\
        0              & I_{3 \times 3}
    \end{bmatrix}
    =
    I_{6 \times 6}
\end{align*}
