\section*{Problem 1}

Prove that given \(R \in S O(3)\) and \(v, w \in \mathbb{R}^{3}\), the following properties hold:
\begin{align*}
    R(v \times w)   & =(R v) \times(R w) \\
    R \hat{w} R^{T} & =\widehat{R w}
\end{align*}

\subsection*{Solution}

\subsubsection*{(a) \( R(v \times w) =(R v) \times(R w) \)}

We have
\[
    SO(3) = \{ R \in \mathbb{R}^{3 \times 3} \mid R R^{T} = I, \det(R) = +1 \}
\]


\subsubsection*{(b) \( R \hat{w} R^{T} =\widehat{R w} \)}

We can show this by the above property.

The hat map is defined as \( \hat{(.)}: \mathbb{R}^{3} \rightarrow \mathbb{R}^{3 \times 3} \) such that
\[
    \hat{v} = \begin{bmatrix}
        0      & -v_{3} & v_{2}  \\
        v_{3}  & 0      & -v_{1} \\
        -v_{2} & v_{1}  & 0
    \end{bmatrix}
\]
for \( v = [v_{1}, v_{2}, v_{3}]^{T} \in \mathbb{R}^{3} \).

Now, for a vector \( v \in \mathbb{R}^{3} \), we have
\[
    R \hat{w} R^{T} v
    =
    R (\hat{w} (R^{T} v))
    =
    R (w \times (R^{T} v))
\]
\[
    \implies
    R (w \times (R^{T} v))
    =
    R w \times R(R^{T} v)
    =
    R w \times (RR^{T}) v
    =
    R w \times v
    =
    (R w) \times v
    =
    \widehat{R w} v
\]
where we used the property that \( R R^{T} = I \).

Hence, \( R \hat{w} R^{T} = \widehat{R w} \).
