\section*{Problem 3}

Given \(\hat{a} \in s o(3)\), Prove that the following relations hold:
\begin{align*}
      & \hat{a}^{2}=a a^{T}-\|a\|^{2} I \\
      & \hat{a}^{3}=-\|a\|^{2} \hat{a}
\end{align*}

\subsection*{Solution}

\subsubsection*{(a) \( \hat{a}^{2}=a a^{T}-\|a\|^{2} I \)}

The skew-symmetric matrix group \( s o(3) \) is defined as
\[
     s o(3) = \{ S \in \mathbb{R}^{3 \times 3} \mid S^{T} = -S \}
\]

Given \( \hat{a} \in s o(3) \), we have
\[
     \hat{a}^{2}
     =
     \hat{a} \hat{a}
     =
     \begin{bmatrix}
          0      & -a_{3} & a_{2}  \\
          a_{3}  & 0      & -a_{1} \\
          -a_{2} & a_{1}  & 0
     \end{bmatrix}
     \begin{bmatrix}
          0      & -a_{3} & a_{2}  \\
          a_{3}  & 0      & -a_{1} \\
          -a_{2} & a_{1}  & 0
     \end{bmatrix}
     =
     \begin{bmatrix}
          -a_{3}^{2}-a_{2}^{2} & a_{1} a_{2}          & a_{1} a_{3}          \\
          a_{1} a_{2}          & -a_{3}^{2}-a_{1}^{2} & a_{2} a_{3}          \\
          a_{1} a_{3}          & a_{2} a_{3}          & -a_{2}^{2}-a_{1}^{2}
     \end{bmatrix}
\]

We can see that this can be written as
\begin{align*}
     \hat{a}^{2}
      & =
     \begin{bmatrix}
          a_{1}^{2}-(a_{1}^{2}+a_{3}^{2}+a_{2}^{2}) & a_{1} a_{2}                               & a_{1} a_{3}                               \\
          a_{1} a_{2}                               & a_{2}^{2}-(a_{1}^{2}+a_{3}^{2}+a_{2}^{2}) & a_{2} a_{3}                               \\
          a_{1} a_{3}                               & a_{2} a_{3}                               & a_{3}^{2}-(a_{1}^{2}+a_{3}^{2}+a_{2}^{2})
     \end{bmatrix}
     \\ & =
     \begin{bmatrix}
          a_{1}^{2}-\|a\|^{2} & a_{1} a_{2}         & a_{1} a_{3}         \\
          a_{1} a_{2}         & a_{2}^{2}-\|a\|^{2} & a_{2} a_{3}         \\
          a_{1} a_{3}         & a_{2} a_{3}         & a_{3}^{2}-\|a\|^{2}
     \end{bmatrix}
     \\ & =
     \begin{bmatrix}
          a_{1}^{2}   & a_{1} a_{2} & a_{1} a_{3} \\
          a_{1} a_{2} & a_{2}^{2}   & a_{2} a_{3} \\
          a_{1} a_{3} & a_{2} a_{3} & a_{3}^{2}
     \end{bmatrix}
     -
     \begin{bmatrix}
          \|a\|^{2} & 0         & 0         \\
          0         & \|a\|^{2} & 0         \\
          0         & 0         & \|a\|^{2}
     \end{bmatrix}
     \\ & =
     a a^{T}-\|a\|^{2} I
\end{align*}
Hence, \( \hat{a}^{2}=a a^{T}-\|a\|^{2} I \).

\subsubsection*{(b) \( \hat{a}^{3}=-\|a\|^{2} \hat{a} \)}

We can show this starting from the above property.

Given \( \hat{a} \in s o(3) \), we have
\[
     \hat{a}^{3}
     =
     \hat{a} \hat{a}^{2}
     =
     \hat{a} (a a^{T}-\|a\|^{2} I)
     =
     \hat{a} a a^{T}-\|a\|^{2} \hat{a}
\]

Now, we know that \( \hat{a} a = a \times a = 0 \) and \( \hat{a} a^{T} = a \times a^{T} = 0 \), since the cross product of a vector with itself is zero.
The result thereby follows.
